ulib/experimental/Steel.Memory.RST.fst
@@ -76,8 +76,8 @@ val frame
   (#inner0:hprop)
   (#a:Type)
   (#inner1:a -> hprop)
-  (delta:hprop{
-    outer0 `equiv` (inner0 `star` delta)})
+  (#[resolve_frame()]
+    delta:hprop{outer0 `equiv` (inner0 `star` delta)})
   (#pre:mem -> prop)
   (#post:mem -> a -> mem -> prop)
   ($f:unit -> Steel a inner0 inner1 pre post)
@@ -91,7 +91,7 @@ val test1 (#a:Type) (r1 r2:ref a) : Steel a
 
 let test1 #a r1 r2 =
   frame (ptr_perm r1 1.0R `star` ptr_perm r2 1.0R)
-        (ptr_perm r2 1.0R)
+//        (ptr_perm r2 1.0R)
         (fun () -> ptr_read r1)
 
 val test2 (#a:Type) (r1 r2:ref a) : Steel a
@@ -103,7 +103,7 @@ val test2 (#a:Type) (r1 r2:ref a) : Steel a
 let test2 #a r1 r2 =
   star_commutative (ptr_perm r1 1.0R) (ptr_perm r2 1.0R);
   let v = frame (ptr_perm r1 1.0R `star` ptr_perm r2 1.0R)
-        (ptr_perm r1 1.0R)
+//        (ptr_perm r1 1.0R)
         (fun () -> ptr_read r2) in
   star_commutative (ptr_perm r1 1.0R) (pts_to r2 1.0R v);
   v
